Actus.lean
@@ -1,7 +1,5 @@
 -- This module serves as the root of the `Actus` library.
 -- Import modules here that should be built as part of the library.
-import «Actus».Basic
-import «Actus».Types
 import «Actus».Types.Classes
 import «Actus».Types.Numbers
 import «Actus».Types.Time
@@ -10,3 +8,4 @@ import «Actus».Types.Automata
 import «Actus».Logic
 import «Actus».Automata
 import «Actus».Contracts
+import «Actus».Basic
