comms/may-2024-actus-dc/source.typ
@@ -1,0 +1,1 @@
+it'd be good to have a section on the different usecases of formal verification, like modeling vs verification of prod code
